Verbatim/memo/concrete3.v
@@ -15,9 +15,9 @@ Module FMemo (STT : state.T) <: MEMO STT.
   Import STT.Defs.
   Import STT.R.Defs.
 
-  Module State_as_UOT <: UsualOrderedType := UOT_from_UCT State_as_UCT.
+  Module Pointer_as_UOT <: UsualOrderedType := UOT_from_UCT Pointer_as_UCT.
   Module Suffix_as_UOT <: UsualOrderedType := List_as_UOT T_as_UOT.
-  Module pair_as_UOT <: UsualOrderedType := Pair_as_UOT State_as_UOT Suffix_as_UOT.
+  Module pair_as_UOT <: UsualOrderedType := Pair_as_UOT Pointer_as_UOT Suffix_as_UOT.
 
   Module FM := FMapAVL.Make pair_as_UOT.
   Module FMF := FMapFacts.Facts FM.
@@ -25,11 +25,12 @@ Module FMemo (STT : state.T) <: MEMO STT.
   Definition Memo : Type := FM.t (option (String * String)).
   Definition emptyMemo : Memo := FM.empty (option (String * String)).
 
-  Definition set_Memo (M : Memo) (stt : State) (sx : String) (o : (option (String * String))) :=
-    FM.add (stt, sx) o M.
+  Definition set_Memo (M : Memo) (pnt : Pointer) (sx : String) (o : (option (String * String))) :=
+    FM.add (pnt, sx) o M.
 
-  Definition get_Memo (M : Memo) (stt : State) (sx : String) : option (option (String * String)) :=
-    FM.find (stt, sx) M.
+  Definition get_Memo (M : Memo) (pnt : Pointer) (sx : String)
+    : option (option (String * String)) :=
+    FM.find (pnt, sx) M.
 
 
   Lemma correct_Memo : forall M stt z o, get_Memo (set_Memo M stt z o) stt z = Some (o).
