Verbatim/memo/impl.v
@@ -49,7 +49,7 @@ Module ImplFn (Import MEM : memo.T).
           (* in a regex approach, transition := derivative *)
           state' := transition a state in
         let
-          lookup := get_Memo M state' s' in
+          lookup := get_Memo M (fst state') s' in
         let
           mpxs :=
           match lookup with
@@ -61,7 +61,7 @@ Module ImplFn (Import MEM : memo.T).
         match mpxs with
         | (M', None) => if (accepting state') then (M' , Some ([a], s')) else
                          if (accepting state) then (M', Some ([], s)) else
-                           ((set_Memo M' state s None), None)
+                           ((set_Memo M' (fst state) s None), None)
         | (M', Some (p, q)) => (M', Some (a :: p, q))
         end
       end.
@@ -104,19 +104,20 @@ Module ImplFn (Import MEM : memo.T).
 
     Module Export MemoEq.
 
-      Lemma lexy_correct : forall M stt z o,
-        lexy M
-        -> get_Memo M stt z = Some (o)
-        -> max_pref_fn z stt = o.
+      Lemma lexy_correct : forall M pnt z o d,
+        lexy M d
+        -> get_Memo M pnt z = Some (o)
+        -> max_pref_fn z (pnt, d) = o.
       Proof.
         intros. unfold lexy in H. apply H in H0. auto.
       Qed.
 
-      Theorem mpref_memo_eq_lexy_F : forall z stt o M M',
-          lexy M
-          -> max_pref_fn__M M z stt = (M', o)
-          -> max_pref_fn z stt = o.
+      Theorem mpref_memo_eq_lexy_F : forall z pnt o M M' d,
+          lexy M d
+          -> max_pref_fn__M M z (pnt, d) = (M', o)
+          -> max_pref_fn z (pnt, d) = o.
       Proof.
+        (*
         induction z; intros.
         - simpl in *. repeat dm; repeat inj_all; auto.
         - simpl in *.
@@ -127,7 +128,10 @@ Module ImplFn (Import MEM : memo.T).
             try(apply lexy_correct in E3; auto; rewrite E3 in E4; auto);
             try(eapply IHz in H; eauto; rewrite E4 in H);
             try(discriminate).
-      Qed.
+          + unfold lexy in H. apply H in E2. rewrite E3 in E4. discriminate.
+          + unfold lexy in H. apply H in E3. rewrite E3 in E4. discriminate.
+      Qed.*)
+      Admitted.
 
       Lemma cons_mprefs__M : forall m Ms z a rules m' Ms' p lst,
           max_prefs__M (m :: Ms) z (a :: rules) = (m' :: Ms', p :: lst)
@@ -137,11 +141,13 @@ Module ImplFn (Import MEM : memo.T).
       Qed.
 
       Theorem mprefs_memo_F : forall z rules Ms Ms' lst,
-          lexy_list Ms
+          lexy_list (zip Ms (map (fun x => snd (snd x)) rules))
           -> length Ms = length rules
           -> max_prefs__M Ms z rules = (Ms', lst)
           -> max_prefs z rules = lst.
       Proof.
+      Admitted.
+        (*
         induction rules; intros.
         - destruct Ms;
             unfold max_prefs__M in H1; simpl in H1; repeat inj_all; subst; auto; discriminate.
@@ -160,29 +166,31 @@ Module ImplFn (Import MEM : memo.T).
               assert(A2 : lexy m).
               { unfold lexy_list in *. apply H. simpl. left. auto. }
               eapply mpref_memo_eq_lexy_F in A2; eauto. subst. auto.
-      Qed.
+      Qed.*)
 
     End MemoEq.
 
     Module Export Accessible.
       
       Lemma acc_helper__M : forall Ms code rules Ms' label o,
-        lexy_list Ms
+        lexy_list (zip Ms (map (fun x => snd (snd x)) rules))
         -> length Ms = length rules
         -> max_of_prefs__M (max_prefs__M Ms code rules) = (Ms', label, o)
         -> max_of_prefs (max_prefs code rules) = (label, o).
       Proof.
+      Admitted.
+        (*
         intros. destruct (max_prefs code rules) eqn:E; destruct (max_prefs__M Ms code rules) eqn:E1.
         - simpl in *. repeat dm; repeat inj_all; subst. eapply mprefs_memo_F in H; eauto.
           + rewrite E in H. subst. simpl in E0. auto.
         - simpl in *. repeat dm; repeat inj_all; subst. eapply mprefs_memo_F in H; eauto.
           rewrite E in H. subst. simpl in E0. auto.
-      Qed.
+      Qed.*)
 
       Lemma acc_recursive_call__M :
         forall code rules label s l suffix Ms Ms',
           Acc lt (length code)
-          -> lexy_list Ms
+          -> lexy_list (zip Ms (map (fun x => snd (snd x)) rules))
           -> length Ms = length rules
           -> max_of_prefs__M (max_prefs__M Ms code rules) = (Ms', label, Some (s :: l, suffix))
           -> Acc lt (length suffix).
@@ -331,10 +339,12 @@ Module ImplFn (Import MEM : memo.T).
 
       Lemma set_Memo_lexy : forall stt0 z0 o o' z stt m,
           max_pref_fn z stt = o'
-          -> lexy m
-          -> get_Memo (set_Memo m stt z o') stt0 z0 = Some o
+          -> lexy m (snd stt)
+          -> get_Memo (set_Memo m (fst stt) z o') (fst stt0) z0 = Some o
           -> max_pref_fn z0 stt0 = o.
       Proof.
+      Admitted.
+        (*
         intros. destruct (String_dec z z0).
         (* originally tried to find an ordering on State *)
         (* realized that was too much, tried to find decidable equality *)
@@ -357,14 +367,16 @@ Module ImplFn (Import MEM : memo.T).
         - assert(stt0 <> stt \/ z0 <> z); auto.
           clear n. eapply correct_Memo_moot in H2; eauto. rewrite H2 in H1.
           eapply lexy_correct; eauto.
-      Qed.
+      Qed.*)
 
       Lemma lexy_closure : 
         forall code stt M o M',
-          lexy M
+          lexy M (snd stt)
           -> max_pref_fn__M M code stt = (M', o)
-          -> lexy M'.
+          -> lexy M' (snd stt).
       Proof.
+      Admitted.
+        (*
         induction code; intros.
         {
           simpl in H0. dm; inv H0; auto.
@@ -401,15 +413,17 @@ Module ImplFn (Import MEM : memo.T).
             unfold lexy. intros.
             eapply set_Memo_lexy; eauto.
         }
-      Qed.
+      Qed.*)
 
       Lemma lexy_list_closure : 
         forall code rules Ms l0 Ms',
-          lexy_list Ms
+          lexy_list (zip Ms (map (fun x => snd (snd x)) rules))
           -> length Ms = length rules
           -> max_prefs__M Ms code rules = (Ms', l0)
-          -> lexy_list Ms'.
+          -> lexy_list (zip Ms' (map (fun x => snd (snd x)) rules)).
       Proof.
+      Admitted.
+        (*
         intros. unfold lexy_list in *. intros M' H2.
         apply In_nth with (d := emptyMemo) in H2. destruct H2 as [n]. destruct H2.
         assert(L := all_lens_const Ms rules code Ms' l0 H0 H1). destruct L.
@@ -433,14 +447,14 @@ Module ImplFn (Import MEM : memo.T).
         rewrite <- Hlen in H2.
         apply nth_In with (d:=emptyMemo) in H2. rewrite H6 in H2. apply H in H2.
         eapply lexy_closure; eauto.
-      Qed.
+      Qed.*)
 
       Lemma lexy_recursive_call_gen :
         forall code rules Ms label o Ms',
-          lexy_list Ms
+          lexy_list (zip Ms (map (fun x => snd (snd x)) rules))
           -> length Ms = length rules
           -> max_of_prefs__M (max_prefs__M Ms code rules) = (Ms', label, o)
-          -> lexy_list Ms'.
+          -> lexy_list (zip Ms' (map (fun x => snd (snd x)) rules)).
       Proof.
         intros. destruct (max_prefs__M Ms code rules) eqn:E.
         assert(l = Ms').
@@ -453,10 +467,10 @@ Module ImplFn (Import MEM : memo.T).
 
       Lemma lexy_recursive_call :
         forall code rules Ms label s l suffix Ms',
-          lexy_list Ms
+          lexy_list (zip Ms (map (fun x => snd (snd x)) rules))
           -> length Ms = length rules
           -> max_of_prefs__M (max_prefs__M Ms code rules) = (Ms', label, Some (s :: l, suffix))
-          -> lexy_list Ms'.
+          -> lexy_list (zip Ms' (map (fun x => snd (snd x)) rules)).
         intros. eapply lexy_recursive_call_gen in H; eauto.
       Qed.
 
@@ -471,7 +485,7 @@ Module ImplFn (Import MEM : memo.T).
              (rules : list (sRule))
              (code : String)
              (Ha : Acc lt (length code))
-             (Hlexy : lexy_list Ms)
+             (Hlexy : lexy_list (zip Ms (map (fun x => snd (snd x)) rules)))
              (Hlen : length Ms = length rules)
              {struct Ha} : (list Memo) * (list Token) * String :=
       match max_of_prefs__M (max_prefs__M Ms code rules) as mpref'
@@ -499,16 +513,16 @@ Module ImplFn (Import MEM : memo.T).
     Definition init_Memos (srules : list sRule) : list Memo :=
       (map (fun x => emptyMemo) srules).
 
-    Lemma lexy_list_cons : forall M Ms,
-        lexy M -> lexy_list Ms -> lexy_list (M :: Ms).
+    Lemma lexy_list_cons : forall M Ms d,
+        lexy M d -> lexy_list Ms -> lexy_list ((M, d) :: Ms).
     Proof.
       intros. unfold lexy_list in *. intros. sis. destruct H1.
-      - subst. auto.
+      - inv H1. auto.
       - apply H0; auto.
     Qed.
 
     Lemma init_Memos_lexy : forall srules,
-        lexy_list (init_Memos srules).
+        lexy_list (zip (init_Memos srules) (map (fun x => snd (snd x)) srules)).
     Proof.
       intros. induction srules.
       - simpl. unfold lexy_list. intros. contradiction.
